Refactored traces to be a fixed vector of optionals

Connect/Breadboard.v
@@ -82,7 +82,7 @@ Module BB.
 
   Open Scope wiring_scope.
 
-  Definition demo1 := List.nil */  zero_rail ~> 0
+  Definition demo1 := [] */  zero_rail ~> 0
                            //  [5] ~> integrator~> 6
                            // [2] ~> integrator~> 3
                            */ incrementor ~> 2
@@ -92,16 +92,16 @@ Module BB.
                            # 3 "Integrated incrementor".
 
   (* Compute (docstring demo1). *)
-  Definition demo2 := List.nil */integrator ~> 9
+  Definition demo2 := [] */integrator ~> 9
                            // [6] ~> delay_5  0 ~> 10.
 
 
 
 
   Definition demo3 bin threshold  :=
-    List.nil // Vector.of_list(seq 0 32) ~> i8051_Component bin threshold dac ~> 32 
+    [] // Vector.of_list(seq 0 32) ~> i8051_Component bin threshold dac ~> 32 
          ~&~
-         List.nil */ zero_rail ~> 0
+         [] */ zero_rail ~> 0
          */ zero_rail ~> 1
          */ zero_rail ~> 2
          */ zero_rail ~> 3
@@ -134,7 +134,9 @@ Module BB.
          */ zero_rail ~> 30
          */ zero_rail ~> 31 .
 
-  Definition run := run.
+  Definition run {l} := @run l.
+
+  Compute (pin_trace_gen demo1).
 
   (* Compute (run demo1 100). *)
   Lemma valid_demo3: valid_wiring (demo3 [0] 6).
