Connect/Wiring.v
@@ -23,28 +23,32 @@ Require Import Ascii.
 Require Import List.
 Require Import ListSet.
 Require Import EqNat.
-Import ListNotations.
 Require Import Arith.
-Open Scope list_scope.
+Require Import Vector.
+Import VectorNotations.
+Open Scope vector_scope.
 
 Require Import IOModule.
 
 Require Import Vector.
 Import Vector.
 Module Wiring.
+  Definition pin := nat.
+  Definition pintrace := fun n c => Vector.t (option (IO.trace c)) n.
+  Definition pinupdate := fun n => Vector.t (option IO.t) n.
   Inductive component :=
-  | watch_set :   forall {n}, Vector.t nat n -> IO.func n -> nat ->  component
-  | just_set : IO.func 1 -> nat -> component
-  | doc :  nat -> string -> component.
-  Definition wiring := list component.
+  | watch_set :   forall {n}, Vector.t pin n -> IO.func n -> pin->  component
+  | just_set : IO.func 1 -> pin -> component
+  | doc :  pin -> string -> component.
+  Definition wiring := fun c => Vector.t component c.
   Notation  "w // m ~> f ~>  n" := ((watch_set m f n) :: w) (at level 80, m at next level) : wiring_scope. 
   Notation  "w */  f ~>  n" := ((just_set f n) :: w) (at level 80, m at next level): wiring_scope. 
-  Notation "w1 ~&~ w2" := (w1 ++ w2) (at level 80) : wiring_scope.
+  Notation "w1 ~&~ w2" := (Vector.append w1 w2) (at level 80) : wiring_scope.
   Notation "w # p c " := ((doc p c)::w) (at level 80, p at level 0) : wiring_scope.
   Open Scope wiring_scope.
 
   Open Scope string_scope.
-  Fixpoint docstring' l acc :=
+  Fixpoint docstring' {c} (l:wiring c) acc :=
     match l with
       | [] => acc
       | w::w' => 
@@ -56,8 +60,8 @@ Module Wiring.
             docstring' w' ("Port Ascii(" ++ n ++ ") "++c ++ "\n" ++ acc)
         end
     end.
-  Definition docstring w := docstring' w "".
-  Fixpoint output_pins l s: set nat :=
+  Definition docstring {c} (w:wiring c) := docstring' w "".
+  Fixpoint output_pins {c} (l:wiring c) s: set pin :=
     let add_i := set_add%nat nat eq_nat_dec in
     match l with
       | [] => s
@@ -71,7 +75,7 @@ Module Wiring.
     end
     end.
 
-  Fixpoint input_pins l s: set nat :=
+  Fixpoint input_pins {c} (l:wiring c) s: set pin :=
     let add_i := set_add%nat nat eq_nat_dec in
     match l with
       | [] => s
@@ -86,29 +90,29 @@ Module Wiring.
         end
     end.
 
-  Fixpoint all_pins' l (s:set nat): set nat :=
+  Fixpoint all_pins {c} (l:wiring c) (s:set pin): set pin :=
     let add_i := set_add%nat nat eq_nat_dec in
     match l with
       | [] => s
       | w::w' =>
     match w with 
       | watch_set n  from fn to =>
-        all_pins' w'
-                  (let new := (to::(to_list from)) in
+        all_pins w'
+                  (let new := (List.cons to (to_list from)) in
                   (List.fold_left (fun se f => add_i f se) s new))
 
-      | just_set  fn to =>  all_pins' w' (add_i to s)
-      | doc  _ _ =>  all_pins' w' s
+      | just_set  fn to =>  all_pins w' (add_i to s)
+      | doc  to _ =>  all_pins w' (add_i to s)
                                end
     end.
-  Definition pins w := all_pins' w List.nil.
+  Definition pins {c} (w:wiring c)  := of_list (all_pins w List.nil).
   (* Checks that all observers have a source and that only one setter per nat *)
-  Fixpoint valid_wiring' l ins outs: Prop :=
+  Fixpoint valid_wiring' {c} (w:wiring c) ins outs: Prop :=
     let add_i := set_add%nat nat eq_nat_dec in
     let notin := (fun el  s => (not (set_In%nat nat  el s))) in
     let union := set_union%nat nat eq_nat_dec in
     let intersect := set_inter%nat nat eq_nat_dec in
-    match l with
+    match w with
       | [] =>
         (* Check that the intersection of inputs and outputs is inputs,
          ie, everything can be read *)
@@ -126,7 +130,7 @@ Module Wiring.
       | doc  _ _ =>  valid_wiring' w'  ins outs
                                    end
     end.
-  Definition valid_wiring w : Prop :=
+  Definition valid_wiring {c} (w: wiring c) : Prop :=
     valid_wiring' w List.nil List.nil.
 
   Require Import Omega.
@@ -146,26 +150,32 @@ Module Wiring.
       | doc  p c =>  
         doc   (p+n) c
     end.
-  Definition rewire w1 w2 :wiring :=
-    let m := List.fold_left max (pins w2) 0 in
-    List.map (wire_add_offset (m+1)) w1.
+  Definition rewire {c c'} (w1: wiring c) {w2 : wiring c'} :wiring c  :=
+    let m := Vector.fold_left max  0 (pins w2)in
+    Vector.map (wire_add_offset (m+1)) w1.
 
-  Theorem rewire_safe : forall w w',
+  Theorem rewire_safe : forall {c c'} (w:wiring c) (w':wiring c'),
                           valid_wiring w ->
                           valid_wiring w' ->
-                          valid_wiring (rewire w w' ~&~ w').
+                          valid_wiring ((@rewire c c' w w') ~&~ w').
     intros.
     induction w.
     auto.
     unfold rewire.
-    assert (H1:forall (A B: Type) (a:A) (b:list A) (f: A-> B) f, List.map f (a::b) = (f a) :: (@List.map A B  f b)).
+    assert (H1:forall (A B: Type) (a:A) c (b:Vector.t A c) (f: A-> B) f, Vector.map f (a::b) = (f a) :: (@Vector.map A B   f c b)).
     intros.
     auto.
     rewrite H1; auto.
 
-    remember (wire_add_offset ((List.fold_left max (pins w') 0)+1)) as f.
+    remember (wire_add_offset ((fold_left max 0 (pins w') )+1)) as f.
     unfold valid_wiring.
     unfold valid_wiring'.
-    admit.
+    remember (f h).
+    case c;
+    unfold append;
+    intros;
+    try split;
+    auto; admit.
+
   Qed.
 End Wiring.
